disk-betree/BlockCacheSystemCrashSafeBlockInterfaceRefinement.dfy
@@ -1,0 +1,17 @@
+include "BlockCacheSystem.dfy"
+include "CrashSafe.dfy"
+
+module BlockCacheSystemCrashSafeBlockInterfaceRefinement {
+  import BCS = BlockCacheSystem
+  import CSBI = CrashSafeBlockInterface
+
+  function Ik(k: BCS.Constants) : CSBI.Constants
+  {
+    CSBI.Constants(k.machine.constants, k.machine.constants)
+  }
+
+  function I(k: BCS.Constants, s: BCS.Variables) : CSBI.Variables
+  {
+    CSBI.Variables(
+  }
+}
